compiler/bootstrap/translation/compiler64ProgScript.sml
@@ -686,7 +686,7 @@ Proof
   \\ simp[FORALL_PROD,EXISTS_PROD]
   \\ conj_tac >- metis_tac[] \\ rw[]
   \\ imp_res_tac stdin_11 \\ rw[]
-  \\ imp_res_tac stdin_get_file_content
+  \\ imp_res_tac stdin_get_fd_content
   \\ xlet_auto >- xsimpl
   \\ xif
   \\ first_x_assum $ irule_at $ Pos hd \\ simp []
@@ -724,7 +724,7 @@ Proof
    (xlet_auto >- (xcon \\ xsimpl)
     \\ rename [‘stdin fs inp pos’]
     \\ ‘stdin_content fs = SOME inp ∧ pos = 0’ by
-     (gvs [stdin_def,get_file_content_def]
+     (gvs [stdin_def,get_fd_content_def]
       \\ fs [stdin_content_def,IS_SOME_EXISTS])
     \\ gvs []
     \\ xlet_auto_spec (SOME openStdIn_spec_str) >- xsimpl
@@ -756,7 +756,7 @@ Proof
   \\ xlet_auto >- (xcon \\ xsimpl)
   \\ rename [‘stdin fs inp pos’]
   \\ ‘stdin_content fs = SOME inp ∧ pos = 0’ by
-    (gvs [stdin_def,get_file_content_def]
+    (gvs [stdin_def,get_fd_content_def]
      \\ fs [stdin_content_def,IS_SOME_EXISTS])
   \\ gvs []
   \\ xlet_auto_spec (SOME openStdIn_spec_str) >- xsimpl
