developers/changes-since-release.md
@@ -31,6 +31,11 @@ BVI now supports multi-arg calls/returns (with a separate constructor).
 `openFile_truncate` has been updated to create files if they are not present,
 better reflecting the implementation of `ffiopen_out` in `basis_ffi.c`.
 
+`get_file_content` has been renamed to `get_fd_content` to better reflect
+its definition and to free up the name for a different definition.
+
+`get_file_content` now defines a function that returns the contents of a file
+(not a file descriptor).
 ### fsFFIProps
 
 `get_mode_fsupdate` has been added and included as a simp:
